WIP: Only spill containing registers.
This also removes mreg families, which we don't need anymore, as well as
some other Bounds lemmas that are no longer interesting.

TODO: Prove that reloading a containing register reloads the subregisters
correctly. This needs a more detailed concept of accessing subregisters in
locmaps and regmaps.

backend/Bounds.v
@@ -43,7 +43,7 @@ Record bounds : Type := mkbounds {
   bound_stack_data_pos: bound_stack_data >= 0;
   used_callee_save_norepet: list_norepet used_callee_save;
   used_callee_save_prop: forall r, In r used_callee_save -> is_callee_save r = true;
-  used_callee_save_closed: forall r, In r used_callee_save -> (forall r', overlap r r' -> In r' used_callee_save)
+  used_callee_save_containing_reg: forall r, In r used_callee_save -> r = containing_reg r
 }.
 
 (** The following predicates define the correctness of a set of bounds
@@ -54,7 +54,7 @@ Section WITHIN_BOUNDS.
 Variable b: bounds.
 
 Definition mreg_within_bounds (r: mreg) :=
-  is_callee_save r = true -> In r (used_callee_save b).
+  is_callee_save r = true -> In (containing_reg r) (used_callee_save b).
 
 Definition slot_within_bounds (sl: slot) (ofs: Z) (ty: typ) :=
   match sl with
@@ -90,14 +90,8 @@ Section BOUNDS.
 
 Variable f: function.
 
-Definition add_regs (u: RegSet.t) (rs: list mreg) : RegSet.t :=
-  fold_left (fun u r => RegSet.add r u) rs u.
-
 Definition record_reg (u: RegSet.t) (r: mreg) : RegSet.t :=
-  if is_callee_save r then
-    let u' := add_regs u (mreg_family r) in
-    RegSet.add r u'
-  else u.
+  if is_callee_save r then RegSet.add (containing_reg r) u else u.
 
 Definition record_regs (u: RegSet.t) (rl: list mreg) : RegSet.t :=
   fold_left record_reg rl u.
@@ -201,46 +195,6 @@ Proof.
   destruct H1. subst a. apply fold_left_preserves; auto. apply IHl; auto.
 Qed.
 
-Remark add_regs_preserves_in:
-  forall l r u,
-  RegSet.In r u -> RegSet.In r (add_regs u l).
-Proof.
-  induction l; simpl; intros. auto. apply IHl.
-  destruct (mreg_eq r a). apply RegSet.add_1; auto. apply RegSet.add_2; auto.
-Qed.
-
-Remark regset_add_swap:
-  forall r a b u,
-  RegSet.In r (RegSet.add a (RegSet.add b u)) -> RegSet.In r (RegSet.add b (RegSet.add a u)).
-Proof.
-  intros. destruct (mreg_eq r a), (mreg_eq r b); auto using RegSet.add_1, RegSet.add_2.
-  apply RegSet.add_3, RegSet.add_3 in H; auto. apply RegSet.add_2, RegSet.add_2; auto.
-Qed.
-
-Remark add_regs_not_in_list:
-  forall l r u,
-  RegSet.In r (add_regs u l) -> ~ In r l -> RegSet.In r u.
-Proof.
-  induction l; simpl; intros. auto.
-  apply Decidable.not_or in H0; destruct H0.
-  apply IHl in H; auto. eapply RegSet.add_3; eauto.
-Qed.
-
-Lemma add_regs_in_list:
-  forall l r u,
-  In r l -> RegSet.In r (add_regs u l).
-Proof.
-  intros. unfold add_regs.
-  apply fold_left_ensures with (b0 := r); auto using RegSet.add_1, RegSet.add_2.
-Qed.
-
-Remark add_regs_split:
-  forall r u l,
-  RegSet.In r (add_regs u l) -> RegSet.In r u \/ In r l.
-Proof.
-  intros. destruct (In_dec mreg_eq r l); eauto using add_regs_not_in_list.
-Qed.
-
 Definition only_callee_saves (u: RegSet.t) : Prop :=
   forall r, RegSet.In r u -> is_callee_save r = true.
 
@@ -248,12 +202,12 @@ Lemma record_reg_only: forall u r, only_callee_saves u -> only_callee_saves (rec
 Proof.
   unfold only_callee_saves, record_reg; intros.
   destruct (is_callee_save r) eqn:CS; auto.
-  destruct (mreg_eq r0 r). subst; auto.
+  destruct (mreg_eq r0 (containing_reg r)). subst; auto.
+  generalize (containing_reg_charact r); intros [EQ | SUB].
+  rewrite <- EQ; auto.
+  generalize (subreg_callee_save r (containing_reg r) SUB); intros.
+  rewrite <- H1; auto.
   apply RegSet.add_3 in H0; auto.
-  apply add_regs_split in H0; destruct H0.
-  auto.
-  apply partitioned_families in H0.
-  eauto using same_family_callee_save.
 Qed.
 
 Lemma record_regs_only: forall rl u, only_callee_saves u -> only_callee_saves (record_regs u rl).
@@ -274,55 +228,42 @@ Proof.
   red; intros. eelim RegSet.empty_1; eauto.
 Qed.
 
-Definition closed_under_families (u: RegSet.t) : Prop :=
-  forall r s, RegSet.In r u -> mreg_family r = mreg_family s -> RegSet.In s u.
+Definition containing_regs_only (u: RegSet.t) : Prop :=
+  forall r, RegSet.In r u -> r = containing_reg r.
 
-Lemma record_reg_closed: forall r u, closed_under_families u -> closed_under_families (record_reg u r).
+Lemma record_reg_containing_only:
+  forall r u, containing_regs_only u -> containing_regs_only (record_reg u r).
 Proof.
-  unfold closed_under_families, record_reg; intros.
+  unfold containing_regs_only, record_reg; intros.
   destruct (is_callee_save r) eqn:CS; eauto.
-
-  assert (Cases: r0 = r \/ mreg_family r0 = mreg_family r \/ RegSet.In r0 u).
-  { destruct (mreg_eq r0 r). left; assumption. right.
-    apply RegSet.add_3 in H0; auto.
-    apply add_regs_split in H0; destruct H0.
-    - right. assumption.
-    - left. apply partitioned_families. assumption. }
-
-  apply RegSet.add_2.
-  destruct Cases as [Eq|[Family|InU]].
-  - subst. apply add_regs_in_list. apply partitioned_families. auto.
-  - apply add_regs_in_list. apply partitioned_families. congruence.
-  - apply add_regs_preserves_in. eauto.
+  destruct (mreg_eq r0 (containing_reg r)). subst; auto.
+  rewrite containing_reg_idempotent; auto.
+  apply RegSet.add_3 in H0; auto.
 Qed.
 
-Lemma record_regs_closed: forall rl u, closed_under_families u -> closed_under_families (record_regs u rl).
+Lemma record_regs_containing_only:
+  forall rl u, containing_regs_only u -> containing_regs_only (record_regs u rl).
 Proof.
-  intros. unfold record_regs. apply fold_left_preserves; auto using record_reg_closed.
+  intros. unfold record_regs. apply fold_left_preserves; auto using record_reg_containing_only.
 Qed.
 
-Lemma record_regs_of_instr_closed: forall u i, closed_under_families u -> closed_under_families (record_regs_of_instr u i).
+Lemma record_regs_of_instr_containing_only:
+  forall u i, containing_regs_only u -> containing_regs_only (record_regs_of_instr u i).
 Proof.
-  intros. destruct i; simpl; auto using record_reg_closed, record_regs_closed.
+  intros. destruct i; simpl; auto using record_reg_containing_only, record_regs_containing_only.
 Qed.
 
-Lemma record_regs_of_function_closed:
-  closed_under_families record_regs_of_function.
+Lemma record_regs_of_function_containing_only:
+  containing_regs_only record_regs_of_function.
 Proof.
   intros. unfold record_regs_of_function.
-  apply fold_left_preserves. apply record_regs_of_instr_closed.
+  apply fold_left_preserves. apply record_regs_of_instr_containing_only.
   red; intros. eelim RegSet.empty_1; eauto.
 Qed.
 
 Lemma in_elements_in_regset: forall r s, In r (RegSet.elements s) -> RegSet.In r s.
 Proof.
   intros. apply RegSet.elements_2. apply InA_alt. exists r; auto.
-Qed.
-
-Lemma in_regset_in_elements: forall r s, RegSet.In r s -> In r (RegSet.elements s).
-Proof.
-  intros. apply RegSet.elements_1 in H. apply InA_alt in H.
-  destruct H. inv H. auto.
 Qed.
 
 Program Definition function_bounds := {|
@@ -352,8 +293,8 @@ Next Obligation.
   apply InA_alt. exists r; auto.
 Qed.
 Next Obligation.
-  apply in_elements_in_regset in H. apply in_regset_in_elements.
-  eauto using overlap_same_family, record_regs_of_function_closed.
+  apply record_regs_of_function_containing_only. apply RegSet.elements_2.
+  apply InA_alt. exists r; auto.
 Qed.
 
 (** We now show the correctness of the inferred bounds. *)
@@ -361,10 +302,9 @@ Qed.
 Lemma record_reg_incr: forall u r r', RegSet.In r' u -> RegSet.In r' (record_reg u r).
 Proof.
   unfold record_reg; intros. destruct (is_callee_save r); auto. apply RegSet.add_2; auto.
-  auto using add_regs_preserves_in.
 Qed.
 
-Lemma record_reg_ok: forall u r, is_callee_save r = true -> RegSet.In r (record_reg u r).
+Lemma record_reg_ok: forall u r, is_callee_save r = true -> RegSet.In (containing_reg r) (record_reg u r).
 Proof.
   unfold record_reg; intros. rewrite H. apply RegSet.add_1; auto.
 Qed.
@@ -374,7 +314,7 @@ Proof.
   intros. unfold record_regs. apply fold_left_preserves; auto using record_reg_incr.
 Qed.
 
-Lemma record_regs_ok: forall r rl u, In r rl -> is_callee_save r = true -> RegSet.In r (record_regs u rl).
+Lemma record_regs_ok: forall r rl u, In r rl -> is_callee_save r = true -> RegSet.In (containing_reg r) (record_regs u rl).
 Proof.
   intros. unfold record_regs. eapply fold_left_ensures; eauto using record_reg_incr, record_reg_ok.
 Qed.
@@ -393,14 +333,14 @@ Definition defined_by_instr (r': mreg) (i: instruction) :=
   | _ => False
   end.
 
-Lemma record_regs_of_instr_ok: forall r' u i, defined_by_instr r' i -> is_callee_save r' = true -> RegSet.In r' (record_regs_of_instr u i).
+Lemma record_regs_of_instr_ok: forall r' u i, defined_by_instr r' i -> is_callee_save r' = true -> RegSet.In (containing_reg r') (record_regs_of_instr u i).
 Proof.
   intros. destruct i; simpl in *; try contradiction; subst; auto using record_reg_ok.
   destruct H; auto using record_regs_incr, record_regs_ok.
 Qed.
 
 Lemma record_regs_of_function_ok:
-  forall r i, In i f.(fn_code) -> defined_by_instr r i -> is_callee_save r = true -> RegSet.In r record_regs_of_function.
+  forall r i, In i f.(fn_code) -> defined_by_instr r i -> is_callee_save r = true -> RegSet.In (containing_reg r) record_regs_of_function.
 Proof.
   intros. unfold record_regs_of_function.
   eapply fold_left_ensures; eauto using record_regs_of_instr_incr, record_regs_of_instr_ok.
@@ -487,17 +427,6 @@ Proof.
   subst r'; auto.
 Qed.
 
-Lemma regset_in_elements:
-  forall u r, RegSet.In r u -> In r (RegSet.elements u).
-Proof.
-  intros. apply RegSet.elements_1 in H.
-  induction (RegSet.elements u).
-  - inversion H.
-  - inversion H.
-    + subst. constructor; auto.
-    + auto using in_cons.
-Qed.
-
 Corollary mreg_within_bounds_diff:
   forall r1 r2,
   mreg_within_bounds function_bounds r1 ->
@@ -507,12 +436,15 @@ Proof.
   intros.
   unfold mreg_diff. split; contradict H0. subst; auto.
   unfold mreg_within_bounds in *; simpl in *. intros.
-  apply overlap_same_family in H0.
-  assert (R1: RegSet.In r1 record_regs_of_function).
-  { apply RegSet.elements_2, In_InA; auto.
-    exploit same_family_callee_save; eauto. }
-  exploit record_regs_of_function_closed; eauto; intros.
-  auto using regset_in_elements.
+  destruct H0 as [SUB | SUB].
+  generalize (subreg_callee_save r1 r2 SUB); intros.
+  apply subreg_of_containing_reg in SUB; subst.
+  rewrite containing_reg_idempotent. apply H.
+  congruence.
+  generalize (subreg_callee_save r2 r1 SUB); intros.
+  apply subreg_of_containing_reg in SUB; subst.
+  rewrite containing_reg_idempotent in H. apply H.
+  congruence.
 Qed.
 
 Lemma slot_is_within_bounds:
